feat: chaining adders (#13)
* chaining

* chain with example

* comments

* nit

DatapathVerification/BitHeap/Examples.lean
@@ -1,6 +1,9 @@
 import DatapathVerification.BitHeap.BitHeap
+import DatapathVerification.BitHeap.Chain
 
 namespace BitHeap
+
+open Chain
 
 namespace Examples
 
@@ -20,6 +23,33 @@ info: { columns := [(0, { elems := Std.HashSet.ofList [] }),
 -/
 #guard_msgs in
 #eval addBitsExample
+
+abbrev BitEnv := Nat → Bool
+
+def fourBitsInCol1 : BitHeap :=
+  let h := BitHeap.empty
+  let h := h.addBit 1 (Circuit.bit 0)
+  let h := h.addBit 1 (Circuit.bit 1)
+  let h := h.addBit 1 (Circuit.bit 2)
+  let h := h.addBit 1 (Circuit.bit 3)
+  h
+
+def compressionChain : List Adder :=
+  [.fullAdder 1 (Circuit.bit 0) (Circuit.bit 1) (Circuit.bit 2)]
+
+-- assign bits 1,2,3 to 1 and bit 0 to 0 => 3 * 2^1 = 6
+/--
+info: 6
+-/
+#guard_msgs in
+#eval fourBitsInCol1.eval (show BitEnv from fun n => n = 1 || n = 2 || n = 3)
+
+-- Result does not change after applying a full adder.
+/--
+info: 6
+-/
+#guard_msgs in
+#eval (applyChain compressionChain fourBitsInCol1).eval (show BitEnv from fun n => n = 1 || n = 2 || n = 3)
 
 end Examples
 
